

# Problem 1

Consider two point masses  $m_1, m_2$  connected by massless rods of lengths  $l_1, l_2$  in a vertical plane.

## Coordinates

$$x_1 = l_1 \sin \phi_1, \quad y_1 = -l_1 \cos \phi_1, \quad (1)$$

$$x_2 = l_1 \sin \phi_1 + l_2 \sin \phi_2, \quad y_2 = -l_1 \cos \phi_1 - l_2 \cos \phi_2 \quad (2)$$

## Velocities

$$\dot{x}_1 = l_1 \dot{\phi}_1 \cos \phi_1, \quad \dot{y}_1 = l_1 \dot{\phi}_1 \sin \phi_1, \quad (3)$$

$$\dot{x}_2 = l_1 \dot{\phi}_1 \cos \phi_1 + l_2 \dot{\phi}_2 \cos \phi_2, \quad \dot{y}_2 = l_1 \dot{\phi}_1 \sin \phi_1 + l_2 \dot{\phi}_2 \sin \phi_2. \quad (4)$$

## Kinetic Energy

$$T = \frac{1}{2}m_1(\dot{x}_1^2 + \dot{y}_1^2) + \frac{1}{2}m_2(\dot{x}_2^2 + \dot{y}_2^2) \quad (5)$$

$$= \frac{1}{2}(m_1 + m_2)l_1^2\dot{\phi}_1^2 + \frac{1}{2}m_2l_2^2\dot{\phi}_2^2 + m_2l_1l_2\dot{\phi}_1\dot{\phi}_2\cos(\phi_1 - \phi_2). \quad (6)$$

## Potential Energy

$$V = -(m_1 + m_2)gl_1 \cos \phi_1 - m_2gl_2 \cos \phi_2. \quad (7)$$

## Lagrangian

$$L = \frac{1}{2}(m_1 + m_2)l_1^2\dot{\phi}_1^2 + \frac{1}{2}m_2l_2^2\dot{\phi}_2^2 + m_2l_1l_2\dot{\phi}_1\dot{\phi}_2\cos(\phi_1 - \phi_2) \\ + (m_1 + m_2)gl_1 \cos \phi_1 + m_2gl_2 \cos \phi_2. \quad (8)$$

## Problem 2

A mass  $m_2$  is attached to a pendulum of length  $l$  and the pendulum is attached to a massless moving pivot moves horizontally with coordinate  $x(t)$ .

### Coordinates

$$x_2 = x + l \sin \phi, \quad (9)$$

$$y_2 = -l \cos \phi. \quad (10)$$

### Velocity

$$\dot{x}_2^2 + \dot{y}_2^2 = \dot{x}^2 + l^2 \dot{\phi}^2 + 2\dot{x}l\dot{\phi} \cos \phi. \quad (11)$$

### Lagrangian

$$\begin{aligned} L = \frac{1}{2}(m_1 + m_2) \dot{x}^2 + \frac{1}{2}m_2 l^2 \dot{\phi}^2 \cos^2 \phi + \frac{1}{2}m_2 l^2 \dot{\phi}^2 \sin^2 \phi \\ + m_2 \dot{x} l \dot{\phi} \cos \phi + m_2 g l \cos \phi. \end{aligned} \quad (12)$$

After simplifying:

$$L = \frac{1}{2}m_1 \dot{x}^2 + \frac{1}{2}m_2 \left( \dot{x}^2 + l^2 \dot{\phi}^2 + 2\dot{x}l\dot{\phi} \cos \phi \right) + m_2 g l \cos \phi. \quad (13)$$

## Problem 3

A simple pendulum of mass  $m$  and length  $l$  whose point of support undergoes prescribed motion.

### General Coordinates

Let  $\phi(t)$  be the angular displacement from the vertical. The coordinates of the pendulum bob are

$$x = x_0(t) + l \sin \phi, \quad (14)$$

$$y = y_0(t) - l \cos \phi. \quad (15)$$

The velocity squared is

$$v^2 = [X^2 + Y^2] = (\dot{x}_0 + l\dot{\phi} \cos \phi)^2 + (\dot{y}_0 + l\dot{\phi} \sin \phi)^2. \quad (16)$$

The Lagrangian is

$$L = \frac{1}{2}m[X^2 + Y^2] - mgY. \quad (17)$$

### (a) Support moving uniformly on a vertical circle

The point of support moves on a vertical circle of radius  $a$  with constant angular frequency  $\gamma$ :

$$x_0 = a \cos(\gamma t), \quad y_0 = a \sin(\gamma t). \quad (18)$$

After substitution and simplification, neglecting total time derivatives, the Lagrangian becomes

$$L = \frac{1}{2}ml^2\dot{\phi}^2 + mal\gamma^2 \cos(\phi - \gamma t) + mgl \cos \phi. \quad (19)$$

### (b) Support oscillating horizontally

The support oscillates horizontally according to

$$x_0 = a \cos(\gamma t), \quad y_0 = 0. \quad (20)$$

The Lagrangian is

$$L = \frac{1}{2}ml^2\dot{\phi}^2 + mal\gamma^2 \cos(\gamma t) \cos \phi + mgl \cos \phi. \quad (21)$$

### (c) Support oscillating vertically

The support oscillates vertically according to

$$y_0 = a \cos(\gamma t), \quad x_0 = 0. \quad (22)$$

The Lagrangian becomes

$$L = \frac{1}{2}ml^2\dot{\phi}^2 + mgl \cos \phi - mal\gamma^2 \cos(\gamma t) \cos \phi. \quad (23)$$